mixfix2/MixfixGrammar2.v
@@ -1,0 +1,97 @@
+From stdpp Require Export list.
+
+Inductive symbol (T : Type) :=
+  | terminal (a : T)
+  | nonterminal.
+
+Global Arguments terminal {_} _.
+Global Arguments nonterminal {_}.
+
+Notation E := nonterminal.
+
+Inductive production (T : Type) :=
+  | small_production : option T → production T
+  | large_production : symbol T → list (symbol T) → symbol T → production T.
+
+Global Arguments small_production {_} _.
+Global Arguments large_production {_} _ _ _.
+
+Definition mixfixgrammar (T : Type) := production T → Prop.
+
+Definition word (T : Type) := list T.
+
+Inductive parse_tree (T : Type) :=
+  | leaf : T → parse_tree T
+  | small_node : production T → option T → parse_tree T
+  | large_node : production T → parse_tree T → parse_list T → parse_tree T → parse_tree T
+
+with parse_list (T : Type) :=
+  | parse_nil : parse_list T
+  | parse_cons : parse_tree T → parse_list T → parse_list T.
+
+Global Arguments leaf {_} _.
+Global Arguments small_node {_} _ _.
+Global Arguments large_node {_} _ _ _ _.
+Global Arguments parse_nil {_}.
+Global Arguments parse_cons {_} _ _.
+
+Scheme parse_tree_list_rec := Induction for parse_tree Sort Prop
+with parse_list_tree_rec := Induction for parse_list Sort Prop.
+
+Scheme parse_tree_list_rec_set := Induction for parse_tree Sort Set
+with parse_list_tree_rec_set := Induction for parse_list Sort Set.
+
+Inductive is_node {T} : parse_tree T → Prop :=
+  | is_small_node p opt_a :
+      is_node (small_node p opt_a)
+  | is_large_node p t1 τ tn :
+      is_node (large_node p t1 τ tn).
+
+Inductive well_formed_parse_tree {T} (g : mixfixgrammar T) : symbol T → parse_tree T → Prop :=
+  | well_formed_leaf a :
+      well_formed_parse_tree g (terminal a) (leaf a)
+  | well_formed_small_node opt_a :
+      g (small_production opt_a) →
+      well_formed_parse_tree g E (small_node (small_production opt_a) opt_a)
+  | well_formed_large_node X1 σ Xn t1 τ tn :
+      g (large_production X1 σ Xn) →
+      well_formed_parse_tree g X1 t1 →
+      well_formed_parse_list g σ τ →
+      well_formed_parse_tree g Xn tn →
+      well_formed_parse_tree g E (large_node (large_production X1 σ Xn) t1 τ tn) 
+
+with well_formed_parse_list {T} (g : mixfixgrammar T) : list (symbol T) → parse_list T → Prop :=
+  | well_formed_parse_nil :
+      well_formed_parse_list g [] parse_nil
+  | well_formed_parse_cons X Xs t ts :
+      well_formed_parse_tree g X t →
+      well_formed_parse_list g Xs ts →
+      well_formed_parse_list g (X :: Xs) (parse_cons t ts).
+
+Scheme well_formed_parse_tree_list_rec := Induction for well_formed_parse_tree Sort Prop
+with well_formed_parse_list_tree_rec := Induction for well_formed_parse_list Sort Prop.
+
+Notation wft g X t := (well_formed_parse_tree g X t).
+Notation wfτ g σ ts := (well_formed_parse_list g σ ts).
+
+Fixpoint yield_tree {T} t : word T :=
+  match t with
+  | leaf a => [a]
+  | small_node p opt_a =>
+      match opt_a with
+      | None => []
+      | Some a => [a]
+      end
+  | large_node p t1 τ tn => yield_tree t1 ++ yield_list τ ++ yield_tree tn 
+  end
+
+with yield_list {T} τ : word T :=
+  match τ with
+  | parse_nil => []
+  | parse_cons t ts => yield_tree t ++ yield_list ts
+  end.
+
+Notation yt t := (yield_tree t).
+Notation yts ts := (yield_list ts).
+
+Definition sentence {T} (g : mixfixgrammar T) w := ∃ t, wft g E t ∧ yt t = w.
