mixfix2/MixfixRepair3.v
@@ -1,0 +1,68 @@
+From disamb Require Export MixfixDisambiguation2.
+From disamb Require Import MyUtils.
+
+Global Instance right_neighborhood_conflict_free_decidable {T} (Q : crules T) p t1 τ tn :
+  Decision (rncf Q p t1 τ tn).
+Proof.
+  unfold rncf.
+  assert (Decision (∀ p2, p CR p2 ∠ Q → ¬ p2 LM tn)). {
+    clear t1 τ. induction tn.
+    - left. intros ???. inv H0.
+    - left. intros ???. inv H0.
+    - destruct (decide (p CR p0 ∠ Q)).
+      + right. intro. eapply H; eauto. constructor.
+      + destruct (decide (∀ p2, p CR p2 ∠ Q → ¬ p2 LM tn1)).
+        * left. intros ???. inv H0. contradiction. eapply n0; eauto.
+        * right. intro. apply n0. intros ???. eapply H; eauto. constructor. assumption. 
+  }
+  destruct (decide (∀ p2 : production T, p CR p2 ∠ Q → ¬ p2 LM tn)).
+  - left. intros ???. inv H1. eapply n; eauto.
+  - right. intro. apply n. intros ???. eapply H0; eauto. constructor. assumption.
+Qed.
+
+Fixpoint repair_cr {T} (Q : crules T) (p : production T)
+    (t1 : parse_tree T) (τ : parse_list T) (tn : parse_tree T) :=
+  if decide (rncf Q p t1 τ tn) then large_node p t1 τ tn else
+  match tn with
+  | large_node pn tn1 τn tnn => large_node pn (repair_cr Q p t1 τ tn1) τn tnn 
+  | _ => (large_node p t1 τ tn)
+  end.
+
+Global Instance left_neighborhood_conflict_free_decidable {T} (Q : crules T) p t1 τ tn :
+  Decision (lncf Q p t1 τ tn).
+Proof.
+  unfold lncf.
+  assert (Decision (∀ p2, p CL p2 ∠ Q → ¬ p2 RM t1)). {
+    clear tn τ. induction t1.
+    - left. intros ???. inv H0.
+    - left. intros ???. inv H0.
+    - destruct (decide (p CL p0 ∠ Q)).
+      + right. intro. eapply H; eauto. constructor.
+      + destruct (decide (∀ p2 : production T, p CL p2 ∠ Q → ¬ p2 RM t1_2)).
+        * left. intros ???. inv H0. contradiction. eapply n0; eauto.
+        * right. intro. apply n0. intros ???. eapply H; eauto. constructor. assumption. 
+  }
+  destruct (decide (∀ p2 : production T, p CL p2 ∠ Q → ¬ p2 RM t1)).
+  - left. intros ???. inv H1. eapply n; eauto.
+  - right. intro. apply n. intros ???. eapply H0; eauto. constructor. assumption.
+Qed.
+
+Fixpoint repair_top {T} (Q : crules T) (p : production T)
+    (t1 : parse_tree T) (τ : parse_list T) (tn: parse_tree T) :=
+  if decide (lncf Q p t1 τ tn) then repair_cr Q p t1 τ tn else
+  match t1 with
+  | large_node p1 t11 τ1 t1n => repair_top Q p1 t11 τ1 (repair_top Q p t1n τ tn)
+  | _ => repair_cr Q p t1 τ tn
+  end.
+
+Fixpoint repair {T} (Q : crules T) (t : parse_tree T) :=
+  match t with  
+  | large_node p t1 τ tn => repair_top Q p (repair Q t1) (repair_list Q τ) (repair Q tn)
+  | _ => t
+  end
+
+with repair_list {T} (Q : crules T) (τ : parse_list T) :=
+  match τ with
+  | parse_nil => parse_nil
+  | parse_cons t ts => parse_cons (repair Q t) (repair_list Q ts)
+  end.
