mixfix2/theorems/MixfixReorderRepair2.v
@@ -1,0 +1,307 @@
+From disamb Require Export MixfixRepair3.
+From disamb Require Import MyUtils.
+From disamb Require Import MixfixRepairWellformed.
+From disamb Require Import MixfixReorderWellformed.
+
+Section MixfixReorderRepair2.
+
+Context {T : Type}.
+Implicit Types (t : parse_tree T) (ts τ : parse_list T) (p : production T) (X : symbol T)
+  (g : mixfixgrammar T) (Xs σ : list (symbol T)) (b : bool) (Q : crules T).
+
+Lemma repair_cr_leftmost_match Q p t1 τ tn :
+  p LM repair_cr Q p t1 τ tn.
+Proof.
+  induction tn as [an|pn opt_an|pn pn1 ? τn pnn]; simpl.
+  - destruct (decide (rncf Q p t1 τ (leaf an))).
+    + constructor.
+    + destruct n. intros ???. inv H0. inv H2.
+  - destruct (decide (rncf Q p t1 τ (small_node pn opt_an))).
+    + constructor.
+    + destruct n. intros ???. inv H0. inv H2.
+  - destruct (decide (rncf Q p t1 τ (large_node pn pn1 τn pnn))).
+    + constructor.
+    + constructor. assumption.
+Qed.
+
+Lemma repair_cr_leftmost_match_2 Q px p t1 τ tn :
+  px LM t1 → px LM repair_cr Q p t1 τ tn.
+Proof.
+  intros. induction tn as [an|pn opt_an|pn pn1 ? τn pnn]; simpl.
+  - destruct (decide (rncf Q p t1 τ (leaf an))).
+    + constructor. assumption.
+    + constructor. assumption.
+  - destruct (decide (rncf Q p t1 τ (small_node pn opt_an))).
+    + constructor. assumption.
+    + constructor. assumption.
+  - destruct (decide (rncf Q p t1 τ (large_node pn pn1 τn pnn))).
+    + constructor. assumption.
+    + constructor. auto.
+Qed.
+
+Lemma repair_cr_assoc Q p1 t11 τ1 p2 t21 τ2 t22 :
+  complete_crules Q → right_dangling p1 → left_dangling p2 →
+  ¬ p2 CL p1 ∠ Q →
+  (∀ p, p1 CR p ∠ Q → ¬ p LM t21) →
+  repair_cr Q p1 t11 τ1 (repair_cr Q p2 t21 τ2 t22) = repair_cr Q p2 (large_node p1 t11 τ1 t21) τ2 t22.
+Proof.
+  intros. induction t22 as [a22|p22 opt_a22|p22 t221 ? τ22 t22n]; intros; simpl.
+  - destruct (decide (rncf Q p2 t21 τ2 (leaf a22))).
+    + destruct (decide (rncf Q p2 (large_node p1 t11 τ1 t21) τ2 (leaf a22))).
+      * simpl. destruct (decide (rncf Q p1 t11 τ1 (large_node p2 t21 τ2 (leaf a22)))).
+        **exfalso. unfold complete_crules in H. apply H with (p2 := p1) in H1; eauto.
+          destruct H1; auto. eapply r1; eauto. constructor. constructor.
+        **destruct t21 as [a21|p21 opt_a21|p21 t211 τ21 t21n]; simpl.
+          ***destruct (decide (rncf Q p1 t11 τ1 (leaf a21))); auto.
+          ***destruct (decide (rncf Q p1 t11 τ1 (small_node p21 opt_a21))); auto.
+          ***destruct (decide (rncf Q p1 t11 τ1 (large_node p21 t211 τ21 t21n))); auto.
+            exfalso. apply n0. intros ???. inv H5. eapply H3; eauto.
+      * destruct n. intros ???. inv H5. inv H7.
+    + destruct n. intros ???. inv H5. inv H7.
+  - destruct (decide (rncf Q p2 t21 τ2 (small_node p22 opt_a22))).
+    + destruct (decide (rncf Q p2 (large_node p1 t11 τ1 t21) τ2 (small_node p22 opt_a22))).
+      * simpl. destruct (decide (rncf Q p1 t11 τ1 (large_node p2 t21 τ2 (small_node p22 opt_a22)))).
+        **exfalso. unfold complete_crules in H. apply H with (p2 := p1) in H1; eauto.
+          destruct H1; auto. eapply r1; eauto. constructor. constructor.
+        **destruct t21 as [a21|p21 opt_a21|p21 t211 τ21 t21n]; simpl.
+          ***destruct (decide (rncf Q p1 t11 τ1 (leaf a21))); auto.
+          ***destruct (decide (rncf Q p1 t11 τ1 (small_node p21 opt_a21))); auto.
+          ***destruct (decide (rncf Q p1 t11 τ1 (large_node p21 t211 τ21 t21n))); auto.
+            exfalso. apply n0. intros ???. inv H5. eapply H3; eauto.
+      * destruct n. intros ???. inv H5. inv H7.
+    + destruct n. intros ???. inv H5. inv H7.
+  - destruct (decide (rncf Q p2 t21 τ2 (large_node p22 t221 τ22 t22n))).
+    + destruct (decide (rncf Q p2 (large_node p1 t11 τ1 t21) τ2 (large_node p22 t221 τ22 t22n))).
+      * simpl. destruct (decide (rncf Q p1 t11 τ1 (large_node p2 t21 τ2 (large_node p22 t221 τ22 t22n)))).
+        **exfalso. unfold complete_crules in H. apply H with (p2 := p1) in H1; eauto.
+          destruct H1; auto. eapply r1; eauto. constructor. constructor.
+        **destruct t21 as [a21|p21 opt_a21|p21 t211 τ21 t21n]; simpl.
+          ***destruct (decide (rncf Q p1 t11 τ1 (leaf a21))); auto.
+          ***destruct (decide (rncf Q p1 t11 τ1 (small_node p21 opt_a21))); auto.
+          ***destruct (decide (rncf Q p1 t11 τ1 (large_node p21 t211 τ21 t21n))); auto.
+            exfalso. apply n0. intros ???. inv H5. eapply H3; eauto.
+      * destruct n. intros ???. inv H5.
+        eapply r; eauto. constructor. assumption.
+    + destruct (decide (rncf Q p2 (large_node p1 t11 τ1 t21) τ2 (large_node p22 t221 τ22 t22n))).
+      * destruct n. intros ???. inv H5. eapply r; eauto. constructor. assumption.
+      * simpl. destruct (decide (rncf Q p1 t11 τ1 (large_node p22 (repair_cr Q p2 t21 τ2 t221) τ22 t22n))).
+        **exfalso. unfold complete_crules in H. apply H with (p1 := p2) in H0; auto.
+          destruct H0; auto. eapply r; eauto. constructor. constructor. apply repair_cr_leftmost_match.
+        **rewrite IHt22_1. reflexivity.
+Qed.
+
+Lemma repair_cr_assoc2 Q p1 t11 τ1 p2 p21 t211 τ21 t21n τ2 t22 :
+  complete_crules Q →
+  (p1 CR p21 ∠ Q ∨ ∃ p, p1 CR p ∠ Q ∧ p LM t211) →
+  repair_cr Q p1 t11 τ1 (repair_cr Q p2 (large_node p21 t211 τ21 t21n) τ2 t22) =
+  repair_cr Q p2 (large_node p21 (repair_cr Q p1 t11 τ1 t211) τ21 t21n) τ2 t22.
+Proof.
+  intro. induction t22 as [a22|p22 opt_a22|p22 t221 ? τ22 t22n]; intros; simpl.
+  - destruct (decide (rncf Q p2 (large_node p21 t211 τ21 t21n) τ2 (leaf a22))).
+    + destruct (decide (rncf Q p2 (large_node p21 (repair_cr Q p1 t11 τ1 t211) τ21 t21n) τ2 (leaf a22))).
+      * simpl. destruct (decide (rncf Q p1 t11 τ1 (large_node p2 (large_node p21 t211 τ21 t21n) τ2 (leaf a22)))).
+        **exfalso. destruct H0.
+          ***eapply r1; eauto. repeat constructor.
+          ***destruct H0 as [p]. inv H0. eapply r1; eauto. repeat constructor. assumption.
+        **destruct (decide (rncf Q p1 t11 τ1 (large_node p21 t211 τ21 t21n))); auto.
+          exfalso. destruct H0.
+          ***eapply r1; eauto. repeat constructor.
+          ***destruct H0 as [p]. inv H0. eapply r1; eauto. repeat constructor. assumption.
+      * destruct n. intros ???. inv H2. inv H4.
+    + destruct n. intros ???. inv H2. inv H4.
+  - destruct (decide (rncf Q p2 (large_node p21 t211 τ21 t21n) τ2 (small_node p22 opt_a22))).
+    + destruct (decide (rncf Q p2 (large_node p21 (repair_cr Q p1 t11 τ1 t211) τ21 t21n) τ2 (small_node p22 opt_a22))).
+      * simpl. destruct (decide (rncf Q p1 t11 τ1 (large_node p2 (large_node p21 t211 τ21 t21n) τ2 (small_node p22 opt_a22)))).
+        **exfalso. destruct H0.
+          ***eapply r1; eauto. repeat constructor.
+          ***destruct H0 as [p]. inv H0. eapply r1; eauto. repeat constructor. assumption.
+        **destruct (decide (rncf Q p1 t11 τ1 (large_node p21 t211 τ21 t21n))); auto.
+          exfalso. destruct H0.
+          ***eapply r1; eauto. repeat constructor.
+          ***destruct H0 as [p]. inv H0. eapply r1; eauto. repeat constructor. assumption.
+      * destruct n. intros ???. inv H2. inv H4.
+    + destruct n. intros ???. inv H2. inv H4.
+  - destruct (decide (rncf Q p2 (large_node p21 t211 τ21 t21n) τ2 (large_node p22 t221 τ22 t22n))).
+    + destruct (decide (rncf Q p2 (large_node p21 (repair_cr Q p1 t11 τ1 t211) τ21 t21n) τ2 (large_node p22 t221 τ22 t22n))).
+      * simpl. destruct (decide (rncf Q p1 t11 τ1 (large_node p2 (large_node p21 t211 τ21 t21n) τ2 (large_node p22 t221 τ22 t22n)))).
+        **exfalso. destruct H0.
+          ***eapply r1; eauto. repeat constructor.
+          ***destruct H0 as [p]. inv H0. eapply r1; eauto. repeat constructor. assumption.
+        **destruct (decide (rncf Q p1 t11 τ1 (large_node p21 t211 τ21 t21n))); auto.
+          exfalso. destruct H0.
+          ***eapply r1; eauto. repeat constructor.
+          ***destruct H0 as [p]. inv H0. eapply r1; eauto. repeat constructor. assumption.
+      * destruct n. intros ???. inv H2. eapply r; eauto. constructor. assumption.
+    + destruct (decide (rncf Q p2 (large_node p21 (repair_cr Q p1 t11 τ1 t211) τ21 t21n) τ2 (large_node p22 t221 τ22 t22n))).
+      * exfalso. apply n. intros ???. inv H2. eapply r; eauto. constructor. assumption.
+      * simpl. destruct (decide (rncf Q p1 t11 τ1 (large_node p22 (repair_cr Q p2 (large_node p21 t211 τ21 t21n) τ2 t221) τ22 t22n))).
+        **exfalso. destruct H0.
+          ***eapply r; eauto. repeat constructor. apply repair_cr_leftmost_match_2. constructor.
+          ***destruct H0 as [p]. inv H0. eapply r; eauto. repeat constructor.
+            apply repair_cr_leftmost_match_2. constructor. assumption.
+        **rewrite IHt22_1; eauto.
+Qed.
+
+Lemma not_rfncf_exists_match Q p t1 τ tn :
+  ¬ rncf Q p t1 τ tn → ∃ px, p CR px ∠ Q ∧ px LM tn.
+Proof.
+  intro. unfold right_neighborhood_conflict_free in H.
+  assert (¬ (∀ p2, p CR p2 ∠ Q → ¬ p2 LM tn)). {
+    intro. destruct H. intros ???. inv H1. apply H0 in H. contradiction.
+  }
+  clear H. induction tn as [an|pn opt_an|pn tn1 ? τn tnn].
+  - destruct H0. intros ???. inv H0.
+  - destruct H0. intros ???. inv H0.
+  - destruct (decide (p CR pn ∠ Q)).
+    + exists pn. split; auto. constructor.
+    + assert (∃ px : production T, p CR px ∠ Q ∧ px LM tn1). {
+        apply IHtn1. intro. destruct H0. intros ???. inv H1; auto. eapply H; eauto.
+      }
+      destruct H as [px]. inv H. exists px. split; auto. repeat constructor. assumption.
+Qed.
+
+Lemma repair_top_repair_cr_assoc g X Q p1 t11 τ1 p2 t21 τ2 t22 :
+  complete_crules Q → right_dangling p1 → left_dangling p2 → wft g X t21 →
+  (∀ p, p1 CL p ∠ Q → ¬ p RM t11) →
+  repair_cr Q p1 t11 τ1 (repair_top Q p2 t21 τ2 t22) = repair_top Q p2 (repair_cr Q p1 t11 τ1 t21) τ2 t22.
+Proof.
+  intro. revert X p1 t11 τ1 p2 τ2 t22. induction t21 as [a21|p21 opt_a21|p21 t211 ? τ21 t21n];
+    intros ??????? HR HL Hwf ?; simpl.
+  - destruct (decide (lncf Q p2 (leaf a21) τ2 t22)).
+    + destruct (decide (rncf Q p1 t11 τ1 (leaf a21))).
+      * simpl. destruct (decide (lncf Q p2 (large_node p1 t11 τ1 (leaf a21)) τ2 t22)).
+        **rewrite repair_cr_assoc; auto.
+          ***intro. eapply l0; eauto. constructor. constructor.
+          ***intros ???. inv H2.
+        **destruct (decide (lncf Q p2 (leaf a21) τ2 t22)); try contradiction.
+          destruct t11 as [a11|p11 opt_a11|p11 t111 τ11 t11n]; simpl.
+          ***destruct (decide (lncf Q p1 (leaf a11) τ1 (repair_cr Q p2 (leaf a21) τ2 t22))); auto.
+          ***destruct (decide (lncf Q p1 (small_node p11 opt_a11) τ1 (repair_cr Q p2 (leaf a21) τ2 t22))); auto.
+          ***destruct (decide (lncf Q p1 (large_node p11 t111 τ11 t11n) τ1 (repair_cr Q p2 (leaf a21) τ2 t22))); auto.
+            exfalso. apply n0. intros ???. inv H2. eapply H0; eauto.
+      * destruct n. intros ???. inv H2. inv H4.
+    + destruct n. intros ???. inv H2. inv H4.
+  - destruct (decide (lncf Q p2 (small_node p21 opt_a21) τ2 t22)).
+    + destruct (decide (rncf Q p1 t11 τ1 (small_node p21 opt_a21))).
+      * simpl. destruct (decide (lncf Q p2 (large_node p1 t11 τ1 (small_node p21 opt_a21)) τ2 t22)).
+        **rewrite repair_cr_assoc; auto.
+          ***intro. eapply l0; eauto. constructor. constructor.
+          ***intros ???. inv H2.
+        **destruct (decide (lncf Q p2 (small_node p21 opt_a21) τ2 t22)); try contradiction.
+          destruct t11 as [a11|p11 opt_a11|p11 t111 τ11 t11n]; simpl.
+          ***destruct (decide (lncf Q p1 (leaf a11) τ1 (repair_cr Q p2 (small_node p21 opt_a21) τ2 t22))); auto.
+          ***destruct (decide (lncf Q p1 (small_node p11 opt_a11) τ1 (repair_cr Q p2 (small_node p21 opt_a21) τ2 t22))); auto.
+          ***destruct (decide (lncf Q p1 (large_node p11 t111 τ11 t11n) τ1 (repair_cr Q p2 (small_node p21 opt_a21) τ2 t22))); auto.
+            exfalso. apply n0. intros ???. inv H2. eapply H0; eauto.
+      * destruct n. intros ???. inv H2. inv H4.
+    + destruct n. intros ???. inv H2. inv H4.
+  - destruct (decide (lncf Q p2 (large_node p21 t211 τ21 t21n) τ2 t22)).
+    + destruct (decide (rncf Q p1 t11 τ1 (large_node p21 t211 τ21 t21n))).
+      * simpl. destruct (decide (lncf Q p2 (large_node p1 t11 τ1 (large_node p21 t211 τ21 t21n)) τ2 t22)).
+        **rewrite repair_cr_assoc; auto.
+          ***intro. eapply l0; eauto. constructor. constructor.
+          ***intros ???. eapply r; eauto. constructor. assumption.
+        **destruct (decide (lncf Q p2 (large_node p21 t211 τ21 t21n) τ2 t22)); try contradiction.
+          destruct t11 as [a11|p11 opt_a11|p11 t111 τ11 t11n]; simpl.
+          ***destruct (decide (lncf Q p1 (leaf a11) τ1 (repair_cr Q p2 (large_node p21 t211 τ21 t21n) τ2 t22))); auto.
+          ***destruct (decide (lncf Q p1 (small_node p11 opt_a11) τ1 (repair_cr Q p2 (large_node p21 t211 τ21 t21n) τ2 t22))); auto.
+          ***destruct (decide (lncf Q p1 (large_node p11 t111 τ11 t11n) τ1 (repair_cr Q p2 (large_node p21 t211 τ21 t21n) τ2 t22))); auto.
+            exfalso. apply n0. intros ???. inv H2. eapply H0; eauto.
+      * simpl. destruct (decide (lncf Q p2 (large_node p21 (repair_cr Q p1 t11 τ1 t211) τ21 t21n) τ2 t22)).
+        **rewrite repair_cr_assoc2; auto. apply not_rfncf_exists_match in n. destruct n as [px]. inv H1.
+          inv H3; auto. right. eauto.
+        **exfalso. apply n0. intros ???. inv H2. eapply l; eauto. constructor. inv H4; constructor. assumption.
+    + destruct (decide (rncf Q p1 t11 τ1 (large_node p21 t211 τ21 t21n))).
+      * simpl. destruct (decide (lncf Q p2 (large_node p1 t11 τ1 (large_node p21 t211 τ21 t21n)) τ2 t22)).
+        **exfalso. apply n. intros ???. inv H2. eapply l; eauto. constructor. constructor. assumption.
+        **destruct (decide (lncf Q p2 (large_node p21 t211 τ21 t21n) τ2 t22)).
+          ***exfalso. apply n. intros ???. inv H2. eapply l; eauto. constructor. assumption.
+          ***destruct t11 as [a11|p11 opt_a11|p11 t111 τ11 t11n]; simpl.
+            ****destruct (decide (lncf Q p1 (leaf a11) τ1 (repair_top Q p21 t211 τ21 (repair_top Q p2 t21n τ2 t22)))); auto.
+            ****destruct (decide (lncf Q p1 (small_node p11 opt_a11) τ1 (repair_top Q p21 t211 τ21 (repair_top Q p2 t21n τ2 t22)))); auto.
+            ****destruct (decide (lncf Q p1 (large_node p11 t111 τ11 t11n) τ1 (repair_top Q p21 t211 τ21 (repair_top Q p2 t21n τ2 t22)))); auto.
+              exfalso. apply n2. intros ???. inv H2. eapply H0; eauto.
+      * simpl. destruct (decide (lncf Q p2 (large_node p21 (repair_cr Q p1 t11 τ1 t211) τ21 t21n) τ2 t22)).
+        **exfalso. apply n. intros ???. inv H2. eapply l; eauto. constructor. inv H4; constructor. assumption.
+        **inv Hwf. erewrite IHt21_1; eauto. inv H7; try constructor. exfalso.
+          apply n0. intros ???. inv H2. inv H4.
+          ***apply conflict_right_well_formed in H1. inv H1. inv H3.
+          ***inv H3.
+Qed.
+
+Lemma repair_top_assoc g X Q p1 t11 τ1 p2 t21 τ2 t22 :
+  complete_crules Q →
+  right_dangling p1 → left_dangling p2 → wft g X (large_node p1 t11 τ1 (large_node p2 t21 τ2 t22)) →
+  repair_top Q p1 t11 τ1 (repair_top Q p2 t21 τ2 t22) = repair_top Q p2 (repair_top Q p1 t11 τ1 t21) τ2 t22.
+Proof.
+  intro. revert X p1 τ1 p2 t21 τ2 t22. induction t11 as [a11|p11 opt_a11|p11 t111 ? τ11 t11n];
+    intros ??????? HL HR Hwft; simpl.
+  - destruct (decide (lncf Q p1 (leaf a11) τ1 (repair_top Q p2 t21 τ2 t22))).
+    + destruct (decide (lncf Q p1 (leaf a11) τ1 t21)).
+      * inv Hwft. inv H8. erewrite repair_top_repair_cr_assoc; eauto. intros ???. inv H1.
+      * destruct n. intros ???. inv H1. inv H3.
+    + destruct n. intros ???. inv H1. inv H3.
+  - destruct (decide (lncf Q p1 (small_node p11 opt_a11) τ1 (repair_top Q p2 t21 τ2 t22))).
+    + destruct (decide (lncf Q p1 (small_node p11 opt_a11) τ1 t21)).
+      * inv Hwft. inv H8. erewrite repair_top_repair_cr_assoc; eauto. intros ???. inv H1.
+      * destruct n. intros ???. inv H1. inv H3.
+    + destruct n. intros ???. inv H1. inv H3.
+  - destruct (decide (lncf Q p1 (large_node p11 t111 τ11 t11n) τ1 (repair_top Q p2 t21 τ2 t22))).
+    + destruct (decide (lncf Q p1 (large_node p11 t111 τ11 t11n) τ1 t21)).
+      * inv Hwft. inv H8. erewrite repair_top_repair_cr_assoc; eauto. intros ???. eapply l0; eauto.
+        constructor. assumption.
+      * destruct n. intros ???. inv H1. eapply l; eauto. constructor. assumption.
+    + destruct (decide (lncf Q p1 (large_node p11 t111 τ11 t11n) τ1 t21)).
+      * destruct n. intros ???. inv H1. eapply l; eauto. constructor. assumption.
+      * inv Hwft. inv H6. inv H8.
+        assert (Xn0 = E). {
+          inv H12; auto. exfalso. apply n. intros ???. inv H1. inv H3.
+          - apply conflict_left_well_formed in H0. inv H0. inv H2.
+          - inv H2.
+        }
+        subst.
+        assert (wft g E
+          (large_node (large_production E σ E) t11n τ1 (large_node (large_production X1 σ1 Xn1) t21 τ2 t22))). {
+          constructor; auto.
+          constructor; auto.
+        }
+        erewrite IHt11n; eauto.
+        erewrite IHt11_1; eauto. constructor. 
+        constructor; auto. constructor; auto.
+        inv HR. apply repair_top_well_formed. constructor; auto.
+Qed.
+
+Lemma reorder_step_repair g X Q t1 t2 :
+  complete_crules Q → wft g X t1 → wft g X t2 → reorder_step t1 t2 → repair Q t1 = repair Q t2.
+Proof.
+  intros. revert H0 H1. revert X. induction H2 using reorder_step_tree_list_rec with
+    (P0 := fun τ τ' H => ∀ Xs, wfτ g Xs τ → wfτ g Xs τ' → repair_list Q τ = repair_list Q τ'); intros; simpl.
+  - inv H0. inv H1. erewrite repair_top_assoc; eauto.
+    + inv H10. constructor.
+    + inv H6. constructor.
+    + constructor; eauto.
+      * apply repair_well_formed. assumption.
+      * apply repair_list_well_formed. assumption.
+      * inv H10. constructor; auto.
+        **apply repair_well_formed. assumption.
+        **apply repair_list_well_formed. assumption.
+        **apply repair_well_formed. assumption.
+  - inv H0. inv H1. erewrite IHreorder_step; eauto.
+  - inv H0. inv H1. erewrite IHreorder_step; eauto.
+  - inv H0. inv H1. erewrite IHreorder_step; eauto.
+  - inv H0. inv H1. erewrite IHreorder_step; eauto.
+  - inv H0. inv H1. erewrite IHreorder_step; eauto.
+Qed.
+
+Lemma reorder_repair g X1 X2 Q t1 t2 :
+  complete_crules Q → wft g X1 t1 → wft g X2 t2 → reorder t1 t2 → repair Q t1 = repair Q t2.
+Proof.
+  intros. induction H2; auto.
+  inv H2.
+  - eapply reorder_step_well_formed in H4 as ?; eauto.
+    rewrite <- IHrtc; auto. erewrite reorder_step_repair; eauto.
+  - eapply reorder_step_well_formed_2 in H4 as ?; eauto.
+    rewrite <- IHrtc; auto. symmetry. erewrite reorder_step_repair; eauto.
+Qed.
+
+End MixfixReorderRepair2.
