mixfix2/theorems/MixfixReorderWellformed.v
@@ -1,0 +1,40 @@
+From disamb Require Export MixfixReorder2.
+From disamb Require Import MyUtils.
+
+Section MixfixReorderWellformed.
+
+Context {T : Type}.
+Implicit Types (t : parse_tree T) (ts τ : parse_list T) (p : production T) (X : symbol T)
+  (g : mixfixgrammar T) (Xs σ : list (symbol T)) (b : bool).
+
+Lemma reorder_step_well_formed g X t1 t2 :
+  wft g X t1 → reorder_step t1 t2 → wft g X t2.
+Proof.
+  intros. revert H. revert X. induction H0 using reorder_step_tree_list_rec with
+    (P0 := fun τ τ' H => ∀ σ, wfτ g σ τ → wfτ g σ τ'); intros.
+  - inv H. inv H8. constructor; auto.
+    assert (X0 = E). { inv H9; inv i; auto. } subst.
+    constructor; auto.
+  - inv H. constructor; auto.
+  - inv H. constructor; auto.
+  - inv H. constructor; auto.
+  - inv H. constructor; auto.
+  - inv H. constructor; auto.
+Qed.
+
+Lemma reorder_step_well_formed_2 g X t1 t2 :
+  wft g X t2 → reorder_step t1 t2 → wft g X t1.
+Proof.
+  intros. revert H. revert X. induction H0 using reorder_step_tree_list_rec with
+    (P0 := fun τ1 τ2 H => ∀ σ, wfτ g σ τ2 → wfτ g σ τ1); intros.
+  - inv H. inv H6. constructor; auto.
+    assert (Xn0 = E). { inv H11; inv i; auto. } subst.
+    constructor; auto.
+  - inv H. constructor; auto.
+  - inv H. constructor; auto.
+  - inv H. constructor; auto.
+  - inv H. constructor; auto.
+  - inv H. constructor; auto.
+Qed.
+
+End MixfixReorderWellformed.
