mixfix2/theorems/MixfixRepairWellformed.v
@@ -1,0 +1,69 @@
+From disamb Require Export MixfixRepair3.
+From disamb Require Import MyUtils.
+
+Section MixfixRepairWellformed.
+
+Context {T : Type}.
+Implicit Types (t : parse_tree T) (ts τ : parse_list T) (p : production T) (X : symbol T)
+  (g : mixfixgrammar T) (Xs σ : list (symbol T)) (b : bool) (Q : crules T).
+
+Lemma repair_cr_well_formed g X Q p t1 τ tn :
+  wft g X (large_node p t1 τ tn) → wft g X (repair_cr Q p t1 τ tn).
+Proof.
+  intro. inv H. revert H5 H6 H7. revert X1 σ t1 τ. induction H8; simpl; intros.
+  - destruct (decide (rncf Q (large_production X1 σ (terminal a)) t1 τ (leaf a))).
+    + constructor; auto. constructor.
+    + destruct n. intros ???. inv H0. inv H2.
+  - destruct (decide (rncf Q (large_production X1 σ E) t1 τ (small_node (small_production opt_a) opt_a))).
+    + constructor; auto. constructor; auto.
+    + destruct n. intros ???. inv H1. inv H3.
+  - destruct (decide (rncf Q (large_production X0 σ0 E) t0 τ0 (large_node (large_production X1 σ Xn) t1 τ tn))).
+    + constructor; auto. constructor; auto.
+    + constructor; auto. inv H8_; auto. exfalso. apply n. intros ???. inv H2. inv H4.
+      * apply conflict_right_well_formed in H1. inv H1. inv H3.
+      * inv H3.
+Qed.
+
+Lemma repair_top_well_formed g X Q p t1 τ t2 :
+  wft g X (large_node p t1 τ t2) → wft g X (repair_top Q p t1 τ t2).
+Proof.
+  intro. inv H. revert H7 H8 H5. revert σ τ t2 Xn. induction H6; intros; simpl.
+  - destruct (decide (lncf Q (large_production (terminal a) σ Xn) (leaf a) τ t2)).
+    + apply repair_cr_well_formed. constructor; auto. constructor.
+    + destruct n. intros ???. inv H0. inv H2.
+  - destruct (decide (lncf Q (large_production E σ Xn) (small_node (small_production opt_a) opt_a) τ t2)).
+    + apply repair_cr_well_formed. constructor; auto. constructor; auto.
+    + destruct n. intros ???. inv H1. inv H3.
+  - destruct (decide (lncf Q (large_production E σ0 Xn0) (large_node (large_production X1 σ Xn) t1 τ tn) τ0 t2)).
+    + apply repair_cr_well_formed. constructor; auto. constructor; auto.
+    + apply IHwell_formed_parse_tree1; auto. inv H6_0; auto. exfalso. apply n.
+      intros ???. inv H2. inv H4.
+      * apply conflict_left_well_formed in H1. inv H1. inv H3.
+      * inv H3.
+Qed.
+
+Lemma repair_well_formed g X Q t :
+  wft g X t → wft g X (repair Q t).
+Proof.
+  intro. induction H using well_formed_parse_tree_list_rec with
+      (P0 := fun σ τ H => wfτ g σ (repair_list Q τ)); simpl.
+  - constructor.
+  - constructor. assumption.
+  - apply repair_top_well_formed. constructor; auto.
+  - constructor.
+  - constructor; auto.
+Qed.
+
+Lemma repair_list_well_formed g σ Q τ :
+  wfτ g σ τ → wfτ g σ (repair_list Q τ).
+Proof.
+  intro. induction H using well_formed_parse_list_tree_rec with
+      (P := fun X t H => wft g X (repair Q t)); simpl.
+  - constructor.
+  - constructor. assumption.
+  - apply repair_top_well_formed. constructor; auto.
+  - constructor.
+  - constructor; auto.
+Qed.
+
+End MixfixRepairWellformed.
